tweaks to fstar logic engine

ModularEngine/src/LogicEngine.FStar/logicEngine.fst
@@ -1,4 +1,3 @@
-﻿#light
 (*
 // *********************************************************
 //
@@ -26,11 +25,11 @@ module LogicEngine
   extern Utilities val _substrateDispatcher_solve : listFS ISubstrateQueryTerm -> listFS substitution -> listFS substitution
 
   val value_knowledge : option IInfostrate -> list term
-	let value_knowledge oi = PrimsListOfList (_value_knowledge (OptionOfPrimsOption oi))
+  let value_knowledge oi = PrimsListOfList (_value_knowledge (OptionOfPrimsOption oi))
   val value_checkSignature : option ISignatureProvider -> term -> principal -> object -> bool
   let value_checkSignature oi t p o = _value_checkSignature (OptionOfPrimsOption oi) t p o
   val substrateDispatcher_solve : list ISubstrateQueryTerm -> list substitution -> list substitution
-	let substrateDispatcher_solve isl sl = PrimsListOfList (_substrateDispatcher_solve (ListOfPrimsList isl) (ListOfPrimsList sl))
+  let substrateDispatcher_solve isl sl = PrimsListOfList (_substrateDispatcher_solve (ListOfPrimsList isl) (ListOfPrimsList sl))
 
   let log = ref ""
   let _freshVarId = ref 0
@@ -50,266 +49,281 @@ module LogicEngine
   val checkJustification : option ISignatureProvider -> term -> option term
   let rec checkJustification _signatureProvider (evidence: term) = 
     match evidence with
-    | App((SignatureEvidence, [Const(PrincipalConstant(ppal)); inf;
-                                Const(SubstrateConstant(signature))])) ->
-      if canSign ppal inf &&
-          value_checkSignature (*!*)_signatureProvider inf ppal signature
-      then
-        Some inf
-      else
-        (* //log.Warn("Spoofed signature {0} from {1} on {2}", signature, ppal, inf) *)
-        None      
-    | App((ModusPonensEvidence, [e1; e2])) ->
-      (match checkJustification _signatureProvider e1, checkJustification _signatureProvider e2 with
-      | Some i1, Some (App((ImpliesInfon, [i1'; i2]))) when i1 = i1' ->
-        Some i2
-      | _ ->
-        (* //log.Warn("Malformed modus ponens proof on {0} and {1}", e1, e2) *)
-        None )
-    | App((AndEvidence, evidences)) ->
-        let infons = collect (fun evidence ->  
-                                    match checkJustification _signatureProvider evidence with
+      | App((SignatureEvidence, [Const(PrincipalConstant(ppal)); inf;
+                                 Const(SubstrateConstant(signature))])) ->
+          if canSign ppal inf &&
+            value_checkSignature (*!*)_signatureProvider inf ppal signature
+          then
+            Some inf
+          else
+            (* //log.Warn("Spoofed signature {0} from {1} on {2}", signature, ppal, inf) *)
+            None      
+      | App((ModusPonensEvidence, [e1; e2])) ->
+          (match checkJustification _signatureProvider e1, checkJustification _signatureProvider e2 with
+             | Some i1, Some (App((ImpliesInfon, [i1'; i2]))) when i1 = i1' ->
+                 Some i2
+             | _ ->
+                 (* //log.Warn("Malformed modus ponens proof on {0} and {1}", e1, e2) *)
+                 None )
+      | App((AndEvidence, evidences)) ->
+          let infons = collect (fun evidence ->  
+                                  match checkJustification _signatureProvider evidence with
                                     | Some i -> [i]
                                     | None -> []) evidences in (* Rk: F# does not need the 'in' *)
-        if length infons = length evidences then
-          Some(App(AndInfon, infons)) (* Rk: no support for |> and <| ? *)
-        else
-          (* //log.Warn("Malformed conjunction proof on {0}", evidence) *)
-          None
-    | App((AsInfonEvidence, [SubstrateQueryTerm(query)])) ->
-        if (not(isEmpty(substrateDispatcher_solve [query] [id]))) then
-          (*Some(App(AsInfon, (SubstrateQueryTerm(query)) :: [])) *) (* Rk: can't build a list as in [1], has to use 1::[] *)
-          Some(App(AsInfon, [ (SubstrateQueryTerm query) ]))
-        else
-          (* //log.Warn("Non-true asInfon evidence at {0}", query) *)
-          None    
-    | ConcretizationEvidence((ev, subst)) ->
-      (match checkJustification _signatureProvider ev with
-      | Some generalProof -> 
-        let concreteProof = match generalProof with
-                            | Forall _ -> instantiate generalProof subst
-                            | _ -> term_apply generalProof subst
-				in
-        Some concreteProof
-      | None -> None) (* Rk: no need for parenthesis or 'in' in F# *)
-    | _ -> 
-      (* //log.Warn("Unhandled evidence type at {0}", evidence) *)
-			None
+            if length infons = length evidences then
+              Some(App(AndInfon, infons)) (* Rk: no support for |> and <| ? *)
+            else
+              (* //log.Warn("Malformed conjunction proof on {0}", evidence) *)
+              None
+      | App((AsInfonEvidence, [SubstrateQueryTerm(query)])) ->
+          if (not(isEmpty(substrateDispatcher_solve [query] [id]))) then
+            (*Some(App(AsInfon, (SubstrateQueryTerm(query)) :: [])) *) (* Rk: can't build a list as in [1], has to use 1::[] *)
+            Some(App(AsInfon, [ (SubstrateQueryTerm query) ]))
+          else
+            (* //log.Warn("Non-true asInfon evidence at {0}", query) *)
+            None    
+      | ConcretizationEvidence((ev, subst)) ->
+          (match checkJustification _signatureProvider ev with
+             | Some generalProof -> 
+                 let concreteProof = match generalProof with
+                   | Forall _ -> instantiate generalProof subst
+                   | _ -> term_apply generalProof subst
+		 in
+                   Some concreteProof
+             | None -> None) (* Rk: no need for parenthesis or 'in' in F# *)
+      | _ -> 
+          (* //log.Warn("Unhandled evidence type at {0}", evidence) *)
+	  None
 
   (*open TranslationfromFStar *)(* Rk: Why can't I do TranslationfromFStar.optionFS on next line?? *)
   let checkJustificationWrapper (s:option ISignatureProvider) (e:term) (*: optionFS term*) =
     OptionOfPrimsOption (checkJustification s e)
 
-	val freshVar : typ -> var
+  val freshVar : typ -> var
   let freshVar (t: typ) =
-	  let name0 = (Concat "SimpleLogicEngine#Var" (string_of_any (read _freshVarId))) in
+    let name0 = (Concat "SimpleLogicEngine#Var" (string_of_any (read _freshVarId))) in
     let ret = {
       name = name0;
       typ = t} in
       (_freshVarId := (!_freshVarId) + 1);
       ret
     
-  val tryDeriveJustification : option IInfostrate -> (substitution * list ISubstrateQueryTerm) -> term -> (term * term) -> list (substitution * (list ISubstrateQueryTerm) * term)
-	val doDeriveJustification  : option IInfostrate -> term -> (substitution * list ISubstrateQueryTerm) -> list (substitution * (list ISubstrateQueryTerm) * term)
-  let rec tryDeriveJustification (_infostrate: option IInfostrate) (pair_subst_conds: substitution * list ISubstrateQueryTerm)
-                             (pr: term) (pair_goal_inf: term * term) =
+  val tryDeriveJustification : option IInfostrate -> (substitution * list ISubstrateQueryTerm) -> term 
+                            -> (term * term) -> list (substitution * (list ISubstrateQueryTerm) * term)
+  val doDeriveJustification  : option IInfostrate -> term -> (substitution * list ISubstrateQueryTerm) 
+                           -> list (substitution * (list ISubstrateQueryTerm) * term)
+
+  let rec tryDeriveJustification 
+      (_infostrate: option IInfostrate) (pair_subst_conds: substitution * list ISubstrateQueryTerm)
+      (pr: term) (pair_goal_inf: term * term) =
     match pair_subst_conds with (subst, conds) -> 
-    match pair_goal_inf with (goal, inf) -> 
-      let straight = function (goal, premise) -> (* Rk: impossible to put types of goal and premise, neigher (goal:term, premise:term) nor (goal, premise) : term * term seem to work  *)
-        (match unifyFrom premise subst goal with
-         | Some s -> [(s, conds, term_apply pr s)]
-         | None -> [] ) in 
-      match inf with
-      | Forall((v, t)) -> (* Rk: 'as' construct not supported *)
-        (match
-          (if domainContains subst v then
-            (match changeVarName inf subst with (newFt, s') ->
-             t, term_apply pr s')
-           else
-            t, pr)
-				 with (i, pr) ->
-          tryDeriveJustification _infostrate (subst, conds) pr (goal, i) ) 
-      | App((ImpliesInfon, [i1; i2])) -> 
-        let v = freshVar Evidence in (* Rk: does not support pairs or triples in the arguments *)
-        let derivePremise subst_conds_goalPr_triple = 
-          let (subst, conds, goalPr) = subst_conds_goalPr_triple in (* Rk: does not seem to be able to parenthesize this match *)
-          let updateProof (subst_conds_premisePr_triple : substitution * (list ISubstrateQueryTerm) * term) : (substitution * (list ISubstrateQueryTerm) * term) = 
-            let (subst, conds, premisePr) = subst_conds_premisePr_triple in
-            let repl = App(ModusPonensEvidence, [premisePr; pr]) in (* TODO: see Builders.fs and Primitives.fs *)
-              ((subst : substitution), 
-               (conds : list ISubstrateQueryTerm),
-               (term_apply goalPr (extend id v repl : substitution) : term)) in 
-          let tmp = doDeriveJustification _infostrate i1 pair_subst_conds in
-            (match pair_subst_conds with (subst, conds) ->
-               map updateProof tmp
-            )
-	in 
-	  append
-          (straight (goal, inf))
-          (collect derivePremise 
-            (tryDeriveJustification _infostrate (subst, conds) (Var v) (goal, i2))) 
-      | inf -> straight (goal, inf)
-    
+      match pair_goal_inf with (goal, inf) -> 
+        let straight = function (goal, premise) -> (* Rk: impossible to put types of goal and premise, neigher (goal:term, premise:term) nor (goal, premise) : term * term seem to work  *)
+          (match unifyFrom premise subst goal with
+             | Some s -> [(s, conds, term_apply pr s)]
+             | None -> [] ) in 
+          match inf with
+            | Forall((v, t)) -> (* Rk: 'as' construct not supported *)
+                (match
+                   (if domainContains subst v then
+                      (match changeVarName inf subst with (newFt, s') ->
+                         t, term_apply pr s')
+                    else
+                      t, pr)
+		 with (i, pr) ->
+                   tryDeriveJustification _infostrate (subst, conds) pr (goal, i) ) 
+            | App((ImpliesInfon, [i1; i2])) -> 
+                let v = freshVar Evidence in (* Rk: does not support pairs or triples in the arguments *)
+                let derivePremise subst_conds_goalPr_triple = 
+                  let (subst, conds, goalPr) = subst_conds_goalPr_triple in (* Rk: does not seem to be able to parenthesize this match *)
+                  let updateProof (subst_conds_premisePr_triple : substitution * (list ISubstrateQueryTerm) * term) : (substitution * (list ISubstrateQueryTerm) * term) = 
+                    let (subst, conds, premisePr) = subst_conds_premisePr_triple in
+                    let repl = App(ModusPonensEvidence, [premisePr; pr]) in (* TODO: see Builders.fs and Primitives.fs *)
+                      ((subst : substitution), 
+                       (conds : list ISubstrateQueryTerm),
+                       (term_apply goalPr (extend id v repl : substitution) : term)) in 
+                  let tmp = doDeriveJustification _infostrate i1 pair_subst_conds in
+                    (match pair_subst_conds with (subst, conds) ->
+                       map updateProof tmp
+                    )
+	        in 
+	          append
+                    (straight (goal, inf))
+                    (collect derivePremise 
+                       (tryDeriveJustification _infostrate (subst, conds) (Var v) (goal, i2))) 
+            | inf -> straight (goal, inf)
+                
   and doDeriveJustification (_infostrate: option IInfostrate) (infon: term) (pair_subst_conds: substitution * list ISubstrateQueryTerm) = 
     match pair_subst_conds with (subst, conds) ->
-    let straight goal =
-      let aux infon = 
-        match infon with
-        | App((JustifiedInfon, [inf; pr])) -> 
-            tryDeriveJustification _infostrate (subst, conds) pr (goal, inf)
-        | _ -> []
-			in
-      collect aux (value_knowledge _infostrate)
-		in
-    (match infon with
-    | App((AsInfon, [ SubstrateQueryTerm(exp) ])) ->
-      (subst, append conds (exp :: []), App(AsInfonEvidence, SubstrateQueryTerm(exp) :: [])) :: []
-    | App((AndInfon, infons)) -> (* TODO: fix the performance decrease *)
-      let parts = 
-        (fold_left 
-          (fun res infon ->
-            fold_right
-              (fun sce_triple res2 -> 
-                let (subst, conds, evLeft) = sce_triple in
-                append 
-								  (fold_right
-                    (fun sce_triple2 res3 ->
-                     let (subst, conds, evRight) = sce_triple2 in
-                      (subst, conds, 
-                       App(AndEvidence, evLeft :: evRight :: [])) :: res3)
-                    (doDeriveJustification _infostrate infon (subst, conds)) []
-                  ) 
-								  res2
-								) res [])
-          ((subst, conds, App(EmptyEvidence, [])) :: []) 
-          infons
-				)
-			in 
-      append (straight infon) []
-    | goal -> straight goal 
-    ) 
+      let straight goal =
+        let aux infon = 
+          match infon with
+            | App((JustifiedInfon, [inf; pr])) -> 
+                tryDeriveJustification _infostrate (subst, conds) pr (goal, inf)
+            | _ -> []
+	in
+          collect aux (value_knowledge _infostrate)
+      in
+        (match infon with
+           | App((AsInfon, [ SubstrateQueryTerm(exp) ])) ->
+               (subst, append conds (exp :: []), App(AsInfonEvidence, SubstrateQueryTerm(exp) :: [])) :: []
+           | App((AndInfon, infons)) -> (* TODO: fix the performance decrease *)
+               let parts = 
+                 (fold_left 
+                    (fun res infon ->
+                       fold_right
+                         (fun sce_triple res2 -> 
+                            let (subst, conds, evLeft) = sce_triple in
+                              append 
+				(fold_right
+                                   (fun sce_triple2 res3 ->
+                                      let (subst, conds, evRight) = sce_triple2 in
+                                        (subst, conds, 
+                                         App(AndEvidence, evLeft :: evRight :: [])) :: res3)
+                                   (doDeriveJustification _infostrate infon (subst, conds)) []
+                                ) 
+				res2
+			 ) res [])
+                    ((subst, conds, App(EmptyEvidence, [])) :: []) 
+                    infons
+		 )
+	       in 
+                 append (straight infon) []
+           | goal -> straight goal 
+        ) 
   
-  
-	val unifyAndSimpl : option substitution -> list (term * term) -> option substitution
-	let rec unifyAndSimpl (s: option substitution) (ts: list (term * term)) = 
-          match ts with
-          | [] -> s
-          | (a, b) :: ts ->
-            (match s with
-              | None -> None
-              | Some s -> unifyAndSimpl (unifyFrom a s b) ts)
+  val unifyAndSimpl : option substitution -> list (term * term) -> option substitution
+  let rec unifyAndSimpl (s: option substitution) (ts: list (term * term)) = 
+    match ts with
+      | [] -> s
+      | (a, b) :: ts ->
+          (match s with
+             | None -> None
+             | Some s -> unifyAndSimpl (unifyFrom a s b) ts)
 
-	val stripPrefix : substitution -> list (term * term) -> list term -> (term -> term) -> ((list term) * term) -> term -> ref (list (substitution * list term)) -> unit
+  val stripPrefix : substitution -> list (term * term) -> list term -> (term -> term) 
+                -> ((list term) * term) -> term -> ref (list (substitution * list term)) -> unit
   let rec stripPrefix subst prefixUnif preconds suff t template res = 
     let immediate = function
       | ([], i) ->
-        (match unifyAndSimpl (Some subst) ((template, i) :: prefixUnif) with
-          | Some subst ->
-            (res := ((subst, preconds) :: (read res)))
-          | None -> ())
+          (match unifyAndSimpl (Some subst) ((template, i) :: prefixUnif) with
+             | Some subst ->
+                 (res := ((subst, preconds) :: (!res)))
+             | None -> ())
       | _ -> () in 
-		(match t with
-    | ((t1 :: pref), App((SaidInfon, t2 :: i :: []))) -> (* Rk: type annotation on t1 not supported *)
-      (match unifyFrom t1 subst t2 with
-        | Some subst -> 
-          stripPrefix subst prefixUnif preconds 
-            (fun i -> suff (App(SaidInfon, t2 :: i :: []))) (pref, i) template res
-        | None ->
-          stripPrefix subst ((t1, t2) :: prefixUnif)
-            preconds (fun i -> suff (App(SaidInfon, t2 :: i :: []))) (pref, i) template res) 
-    | (pref, App((AndInfon, infons))) ->
-      iterate (fun infon -> 
-                  stripPrefix subst prefixUnif preconds suff (pref, infon) template res) infons
-    | (pref, App((ImpliesInfon, a :: b :: []))) ->
-        immediate t;
-        stripPrefix subst prefixUnif (suff a :: preconds) suff (pref, b) template res
-    | (pref, Var v) when domainContains subst v ->
-      stripPrefix subst prefixUnif preconds suff (pref, subst_apply subst v) template res
-    | t -> immediate t)
+      (match t with
+         | ((t1 :: pref), App((SaidInfon, [t2;i]))) -> (* Rk: type annotation on t1 not supported *)
+             (match unifyFrom t1 subst t2 with
+                | Some subst -> 
+                    stripPrefix subst prefixUnif preconds 
+                      (fun j -> suff (App(SaidInfon, [t2;j]))) (pref, i) template res
+                | None ->
+                    stripPrefix subst ((t1, t2) :: prefixUnif)
+                      preconds (fun j -> suff (App(SaidInfon, [t2;j]))) (pref, i) template res) 
+         | (pref, App((AndInfon, infons))) ->
+             iterate (fun infon -> 
+                        stripPrefix subst prefixUnif preconds suff (pref, infon) template res) infons
+         | (pref, App((ImpliesInfon, a :: b :: []))) ->
+             immediate t;
+             stripPrefix subst prefixUnif (suff a :: preconds) suff (pref, b) template res
+         | (pref, Var v) when domainContains subst v ->
+             stripPrefix subst prefixUnif preconds suff (pref, subst_apply subst v) template res
+         | t -> immediate t)
 
   let infonsWithPrefix (_infostrate: option IInfostrate) (subst: substitution) (pref: list term) (template: term) =
     let res = ref [] in
-    iterate (fun k -> stripPrefix subst [] [] (fun x -> x) (pref, k) template res) 
-      (value_knowledge _infostrate);
-    read res
+      iterate (fun k -> stripPrefix subst [] [] (fun x -> x) (pref, k) template res) 
+        (value_knowledge _infostrate);
+      !res
     
-  val doDerive : option IInfostrate -> list term -> (substitution * list ISubstrateQueryTerm) -> term -> list (substitution * list ISubstrateQueryTerm)
-  val checkOne : option IInfostrate -> ( ((substitution * list ISubstrateQueryTerm) * list term ) -> list (substitution * list ISubstrateQueryTerm))
-  let rec doDerive (_infostrate: option IInfostrate) (pref: list term) 
-               (pair_subst_conds: substitution * list ISubstrateQueryTerm)
-               (infon: term) = 
-    match pair_subst_conds with (subst, conds) -> (* Rk: does not support patterns in formal parameters *)
-    (match infon with
-    | App((AndInfon, infons)) -> 
-        fold_left (fun substs infon ->
-                  collect 
-                    (fun s -> doDerive _infostrate pref s infon) substs
-                ) ((subst, conds) :: []) infons
-    | App((EmptyInfon, []))-> 
-      (subst, conds) :: []
-    | App((SaidInfon, [ppal; infon])) ->
-      doDerive _infostrate (ppal :: pref) (subst, conds) infon
-    | Var(v) when domainContains subst v ->
-      doDerive _infostrate pref (subst, conds) (subst_apply subst v)
-    | App((AsInfon, [SubstrateQueryTerm(exp)])) ->
-      if isEmpty pref then
-        (subst, append conds (exp :: [])) :: []
-      else
-        failwith "asInfon(...) under prefix"
-    | App((JustifiedInfon, [inf; ev])) when pref = [] ->
-        let unifyEv triple_scp =
-          (match triple_scp with (subst', conds', pr') ->
-          (match unifyFrom ev subst' pr' with
-            | Some s -> let x = (append conds conds' : list ISubstrateQueryTerm) in
-                        (s, x) :: [] 
-            | None -> ([] : list (substitution * list ISubstrateQueryTerm) ))) in
-      collect unifyEv (doDeriveJustification _infostrate inf (subst, conds))
-    | templ ->
-      collect (checkOne _infostrate) (map 
-        (fun s_ps_pair -> let (s, ps) = s_ps_pair in ((s, conds), ps)) 
-        (infonsWithPrefix _infostrate subst pref templ : list (substitution * list term)))
-    )
+  val doDerive : option IInfostrate -> list term -> (substitution * list ISubstrateQueryTerm) -> term 
+              -> list (substitution * list ISubstrateQueryTerm)
+  val checkOne : option IInfostrate -> ( ((substitution * list ISubstrateQueryTerm) * list term )
+              -> list (substitution * list ISubstrateQueryTerm))
 
-  and checkOne _infostrate = function
-      | (substConds, pre :: pres) -> 
+  (*  Given a prefix (list of principal ITerms) a current Substitution with  *)
+  (*  side conditions (AsInfo ITerms) and a target infon ITerm to derive *)
+  (*  this method will recursively derive the target infon depending on its *)
+  (*  structure. *)
+  let rec doDerive (_infostrate: option IInfostrate) (pref: list term) (* pref is a prefix of principals p said q said ... *) 
+      (pair_subst_conds: substitution * list ISubstrateQueryTerm)
+      (infon: term) = (* infon is the target *)
+    let (subst, conds)= pair_subst_conds in  (* Rk: does not support patterns in formal parameters *)
+      match infon with
+        | App((AndInfon, infons)) -> 
+            (* Q: this fold_left indicates that the returned list is order insensitive *)
+            fold_left (fun substs infon ->
+                         collect 
+                           (fun s -> doDerive _infostrate pref s infon) substs)
+              ((subst, conds) :: []) infons
+        | App((EmptyInfon, []))-> 
+            (subst, conds) :: []
+        | App((SaidInfon, [ppal; infon])) ->
+            doDerive _infostrate (ppal :: pref) (subst, conds) infon
+        | Var(v) when domainContains subst v ->
+            doDerive _infostrate pref (subst, conds) (subst_apply subst v)
+        | App((AsInfon, [SubstrateQueryTerm(exp)])) ->
+            if isEmpty pref 
+            then [(subst, append conds [exp])] (* Q: why not cons? seems to be order sensitive here. *)
+            else failwith "asInfon(...) under prefix"
+        | App((JustifiedInfon, [inf; ev])) when pref = [] ->
+            let unifyEv triple = 
+              let (subst', conds', pr') = triple in
+                match unifyFrom ev subst' pr' with
+                  | Some s ->                      (*                       let x = (append conds conds' : list ISubstrateQueryTerm) in *)
+                      let x = append conds conds' in 
+                        [(s, x)]
+                  | None -> [] in 
+              (* ([] : list (substitution * list ISubstrateQueryTerm) )) in *)
+              collect unifyEv (doDeriveJustification _infostrate inf (subst, conds))
+        | templ ->
+            (* Rk: Bug? We really should have a nested let rec *)
+            (*             let rec checkOne = function *)
+            (*               | (substConds, pre :: pres) ->  *)
+            (*                   collect (fun s -> checkOne (s, pres)) (doDerive _infostrate [] substConds pre) *)
+            (*               | (substConds, []) -> *)
+            (*                   substConds :: [] in *)
+            collect 
+              (checkOne _infostrate) 
+              (map 
+                 (fun (s, ps) -> ((s, conds), ps))
+                 (infonsWithPrefix _infostrate subst pref templ)) (*  : list (substitution * list term))) *)
+                
+and checkOne _infostrate = function
+    | (substConds, pre :: pres) ->
         collect (fun s -> checkOne _infostrate (s, pres)) (doDerive _infostrate [] substConds pre)
-      | (substConds, []) ->
+    | (substConds, []) ->
         substConds :: []
   
-  val my_append : list 'a -> list 'a -> list 'a
-  let my_append l1 l2 = append l1 l2
-
   let derive (_infostrate: option IInfostrate) (target: term) (substs: list substitution) : list substitution =
     fold_right
       (fun subst res ->
-			  my_append
-        (fold_right
-          (fun subst_conds_pair res2 -> let (subst, conds) = subst_conds_pair in
-            my_append (substrateDispatcher_solve conds (subst :: [])) res2)
-          (doDerive _infostrate [] (subst, []) (target)) []
-        ) res
-			)
+	 append
+           (fold_right
+              (fun (subst, conds) res2 -> 
+                 append (substrateDispatcher_solve conds ([subst])) res2)
+              (doDerive _infostrate [] (subst, []) (target)) [])
+           res)
       substs []
-
+      
   let deriveWrapper (_i: option IInfostrate) (t: term) (s: list substitution) (*: (TranslationfromFStar.listFS substitution) *)=
     (ListOfPrimsList (derive _i t s) (* : TranslationfromFStar.listFS substitution *)) (* Rk: cannot seem to annotate with type *)
 
-  let deriveJustification (_infostrate: option IInfostrate) (infon: term) (proofTemplate: term)
-                          (substs: list substitution) : list substitution =
+  let deriveJustification 
+      (_infostrate: option IInfostrate) (target: term) (proofTemplate: term)
+      (substs: list substitution) : list substitution =
     fold_right
       (fun subst res -> 
-			  my_append
-        (fold_right
-          (fun subst_conds_proof_triple res2 -> let (subst, conds, proof) = subst_conds_proof_triple in
-					  my_append
-            (match unifyFrom proof subst proofTemplate with
-              | Some subst -> substrateDispatcher_solve conds (subst :: [])
-              | None -> []
-            ) 
-						res2)
-          (doDeriveJustification _infostrate infon (subst, [])) []
-        )
-			  res)
+	 append
+           (fold_right
+              (fun (subst, conds, proof) res2 -> 
+		 append (* Note: much like derive, except we check that ...  *)
+                   (match unifyFrom proof subst proofTemplate with (* ... the proof found is compatible with the proof template requested *)
+                      | Some subst -> substrateDispatcher_solve conds [subst]
+                      | None -> [])
+		   res2)
+              (doDeriveJustification _infostrate target (subst, [])) [])
+	   res)
       substs []
       
   let deriveJustificationWrapper (_i: option IInfostrate) (i: term) (p: term) (s: list substitution) (*: listFS substitution*) =
